nola/examples/heap_lang/total_adequacy.v
@@ -5,20 +5,21 @@ From nola.examples.heap_lang Require Export adequacy.
 From nola.examples.heap_lang Require Import proofmode notation.
 From iris.prelude Require Import options.
 
-Definition heap_total Σ `{!heapGpreS Σ} X W s e σ φ :
-  (∀ `{!heapGS_gen HasNoLc Σ X W}, ⊢ inv_heap_inv -∗ WP e @ s; ⊤ [{ v, ⌜φ v⌝ }]) →
-  (∀ `{!invGS_gen HasNoLc Σ}, ⊢ |={⊤}=> ∃ x, W x) → sn erased_step ([e], σ).
+Definition heap_total Σ `{!heapGpreS Σ} s e σ φ :
+  (∀ `{!heapGS_gen HasNoLc Σ}, ⊢ |==> ∃ W, let _ := HeapWGS _ W in
+    W ∗ (inv_heap_inv -∗ WP e @ s; ⊤ [{ v, ⌜φ v⌝ }])) →
+  sn erased_step ([e], σ).
 Proof.
-  intros Hwp Winit. eapply (twp_total _ _). iIntros (?).
-  iMod Winit as (x) "W". iMod (gen_heap_init σ.(heap)) as (?) "[Hh _]".
+  intros Hwp; eapply (twp_total _ _); iIntros (?) "".
+  iMod (gen_heap_init σ.(heap)) as (?) "[Hh _]".
   iMod (inv_heap_init loc (option val)) as (?) ">Hi".
   iMod (proph_map_init [] σ.(used_proph_id)) as (?) "Hp".
   iMod (mono_nat_own_alloc 0) as (γ) "[Hsteps _]".
-  iModIntro.
+  iMod (Hwp (HeapGS _ _ _ _ _ _)) as (W) "[W Hwp]". iModIntro.
   iExists
-    (λ σ ns κs _, (W x ∗ gen_heap_interp σ.(heap) ∗
+    (λ σ ns κs _, (W ∗ gen_heap_interp σ.(heap) ∗
                    proph_map_interp κs σ.(used_proph_id) ∗
                    mono_nat_auth_own γ 1 ns)%I),
     id, (λ _, True%I), _; iFrame.
-  by iApply (Hwp (HeapGS _ _ _ _ _ _ _ _ _ _ _)).
+  by iApply "Hwp".
 Qed.
